WIP so I don't break things forever

coq-verification/src/Concrete/MM/Proofs.v
@@ -2,6 +2,7 @@ Require Import Coq.Arith.PeanoNat.
 Require Import Coq.Lists.List.
 Require Import Coq.micromega.Lia.
 Require Import Coq.NArith.BinNat.
+Require Import Coq.omega.Omega.
 Require Import Hafnium.AbstractModel.
 Require Import Hafnium.Concrete.Datatypes.
 Require Import Hafnium.Concrete.Notations.
@@ -43,6 +44,8 @@ Section Proofs.
       rewrite (surjective_pairing x) in H
     | _ => break_match
     | _ => solver
+    | H : break = continue |- _ => cbv [break continue] in H; solver
+    | H : continue = break |- _ => cbv [break continue] in H; solver
     end.
   Ltac simplify := repeat simplify_step.
 
@@ -114,38 +117,145 @@ Section Proofs.
   Lemma mm_map_level_table_attrs conc begin end_ pa attrs table level
         flags ppool :
     let ret :=
-        mm_map_level conc begin end_ pa attrs table level flags ppool in
+        mm_map_level conc begin end_ pa attrs table (level-1) flags ppool in
     let success := fst (fst (fst ret)) in
     let table := snd (fst (fst ret)) in
     let conc' := snd (fst ret) in
     let ppool' := snd ret in
-    let begin : nat := mm_index begin level in
-    let end_ : nat := mm_index end_ level in
-    has_uniform_attrs conc'.(ptable_deref) table level attrs begin end_.
+    has_uniform_attrs conc.(ptable_deref) table (level - 1) attrs begin end_.
   Admitted.
 
   (* placeholder; later there will be actual expressions for the new abstract
      states *)
   Axiom TODO : @abstract_state paddr_t nat.
 
-  (* TODO: we know that all the mm_map_level steps succeed because we
-  know that the whole thing succeeds. But how do we use that in the
-  invariant? *)
+
+  (* Need to figure out alignment situation!
+     - condition of while loop is [end <= begin]
+     - [end] is rounded *up* to the nearest page
+     - [mm_start_of_next_block]...what does it do? I think it gets the address of
+       the next table entry at the given level, as suggested by incrementation of
+       [table_index]
+        * it zeroes out all the bits below the provided block size, which is mm_entry_size level, so yes
+     
+     if [end] is not aligned to the entry size, then what will happen?
+        well, we'll eventually get to a point where [mm_index begin level = mm_index end level], but begin < end because begin is aligned
+        we'll do that reassignment and the range checks will keep things honest
+        then mm_index begin level = S (mm_index end level) and begin >= end; break
+
+     if [end] is aligned, then what will happen?
+        as soon as [mm_index begin level = mm_index end level], [begin = end] and we break
+
+     so...while_loop_end_exact is NOT the right thing, quite. We don't get
+     [begin = end_]; we get [begin >= end_] and
+     [mm_index begin level = if end_aligned_to_entry_size
+                             then mm_index end level
+                             else S (mm_index end level) ]
+     
+     if we know [mm_index begin level <= S (mm_index end level)], does that help?
+
+   *)
+
+  (* maybe we need some part of the concrete state to say where each
+  ptable_pointer is, exactly one location. They can be either in mpool
+  or somewhere in a page table, but this would enforce by construction
+  that they're not repeated... *)
+  Axiom pointer_in_table :
+    (Datatypes.ptable_pointer -> mm_page_table) ->
+    Datatypes.ptable_pointer -> mm_page_table -> Prop.
+
+
+  Definition deref_noncircular (c : concrete_state) : Prop :=
+    forall ptr,
+      ~ pointer_in_table c.(ptable_deref) ptr (c.(ptable_deref) ptr).
+
+  Axiom mpool_contains : mpool -> Datatypes.ptable_pointer -> Prop.
+
+  Definition pointers_ok (c : concrete_state) (ppool : mpool) : Prop :=
+    deref_noncircular c
+    /\ (forall ptr,
+           mpool_contains ppool ptr <->
+           (forall ptr2, ~ pointer_in_table c.(ptable_deref) ptr (c.(ptable_deref) ptr2))).
+
+  (* TODO : is this the right approach? *)
+  Lemma mm_map_level_noncircular c begin end_ pa attrs ptr level flags ppool :
+    pointers_ok c ppool ->
+    let ret := mm_map_level
+                 c begin end_ pa attrs (ptable_deref c ptr) level flags ppool in
+    let table := snd (fst (fst ret)) in
+    ~ pointer_in_table (ptable_deref c) ptr table.
+  Admitted. (* TODO *)
+ 
+  Definition is_start_of_block (a : ptable_addr_t) (level : nat) : Prop :=
+    (a & (mm_entry_size level - 1))%N = 0.
+
+  Lemma mm_start_of_next_block_is_start a level :
+    is_start_of_block (mm_start_of_next_block a (mm_entry_size level)) level.
+  Admitted. (* TODO *)
+
+  (* dumb wrapper for one of the invariants so it doesn't get split too early *)
+  Definition is_begin_or_block_start
+             (start_begin begin : ptable_addr_t) root_level : Prop :=
+      (begin = start_begin \/ is_start_of_block begin root_level).
+
+  (* TODO: we're not actually using the starting concrete state all
+  the time; the concrete state has to change. But how exactly can we
+  encode that? *)
+  (* In reality, it shouldn't matter that the concrete state is
+  changing because we only care about the subset of it that leads to
+  the pointers we're changing, and those pointers should all be on the
+  same level and not be in each other's paths. Can we encode this by
+  passing in the index sequences to the pointer, perhaps, instead of
+  the entire concrete state? *)
+  (* Can we say each pointer has exactly one index sequence and they
+  don't affect each other's index sequences and then pass in an index
+  sequence to abstract_reassign_pointer instead of a concrete state
+  and a pointer? *)
+  (* Should we do away with ptable_pointer entirely? *)
+  (* what if, instead of ptable_pointer, we had something that
+  indicated position-from-root? Something like the index sequences? *)
+  (* the beauty of the current solution is that it *does* remap every
+  location exactly as happens in concrete state. But can we preserve
+  that beauty? Where exactly would we run into problems with allowing
+  for repeats of the same pointer? *)
+  (* well, somewhere we need to know that the concrete state doesn't
+  change stuff in random other places...we *need* the property that
+  ptable_pointers don't repeat themselves *)
+  (* in this case, that reasoning would look like:
+     - every ptable_pointer has exactly one index_sequence from exactly one table (reassign_pointer preserves that property because mm_map_level output fits certain conditions)
+     - none of the reassignments we do will change each other's index sequence, because they can't change anything shorter than themselves
+     - if the index_sequence for the pointer passed into abstract_reassign_pointer hasn't changed, we can switch out concrete states
+   *)
   Definition mm_map_root_loop_invariant
-             start_abst start_conc t_ptrs start_begin attrs root_level
+             start_abst start_conc t_ptrs start_begin end_ attrs root_level
              (state : concrete_state * ptable_addr_t * size_t * bool * mpool)
     : Prop :=
     let '(s, begin, table_index, failed, ppool) := state in
-    let index := mm_index begin root_level in
-    table_index = index /\
+    let index := table_index - mm_index start_begin root_level in
+    let end_index := mm_index end_ root_level in
     (failed = true \/
-     represents
-       (fold_right
-          (fun t_ptr abst =>
-             abstract_reassign_pointer abst start_conc t_ptr attrs start_begin index)
-          start_abst
-          (firstn table_index t_ptrs))
-       s).
+     (table_index = mm_index begin root_level
+      /\ (start_begin <= begin)%N
+      /\ (begin <= mm_level_end end_ root_level)%N
+      /\ pointers_ok s ppool
+      /\ is_begin_or_block_start start_begin begin root_level
+      /\ (Forall (fun t_ptr =>
+                    Forall
+                      (fun root_ptr =>
+                         index_sequences_to_pointer
+                           start_conc.(ptable_deref) t_ptr root_ptr
+                         = index_sequences_to_pointer
+                             s.(ptable_deref) t_ptr root_ptr)
+                      (hafnium_root_ptable :: map vm_root_ptable vms))
+                 t_ptrs)
+      /\ (represents
+            (fold_left
+               (fun abst t_ptr =>
+                  abstract_reassign_pointer
+                    abst start_conc t_ptr attrs start_begin end_)
+               (firstn index t_ptrs)
+               start_abst)
+            s))).
 
   (* TODO: move *)
   Lemma N_lnot_0_r a : N.lnot a 0 = a.
@@ -209,6 +319,162 @@ Section Proofs.
        precondition in terms of mm_level_end. *)
   Admitted.
 
+  Lemma mm_index_le_mono a b level :
+    (a <= b)%N ->
+    (b <= mm_level_end a level)%N ->
+    mm_index a level <= mm_index b level.
+  Admitted. (* TODO *)
+
+  (* TODO: move *)
+  Lemma firstn_snoc {A} i ls d :
+    i < length ls ->
+    @firstn A (S i) ls = firstn i ls ++ (nth_default d ls i :: nil).
+  Admitted. (* TODO *)
+
+  (* TODO: move *)
+  Lemma abstract_reassign_pointer_for_entity_change_concrete
+        abst conc conc' ptr owned valid e root_ptr begin end_ :
+    index_sequences_to_pointer conc.(ptable_deref) ptr root_ptr
+    = index_sequences_to_pointer conc'.(ptable_deref) ptr root_ptr ->
+    abstract_reassign_pointer_for_entity
+      abst conc ptr owned valid e root_ptr begin end_
+    = abstract_reassign_pointer_for_entity
+        abst conc' ptr owned valid e root_ptr begin end_.
+  Proof.
+    cbv beta iota delta [abstract_reassign_pointer_for_entity].
+    intro Heq. rewrite Heq. reflexivity.
+  Qed.
+
+  (* TODO : move *)
+  Lemma fold_right_ext {A B} (f g : A -> B -> B) b ls :
+    (forall a b, In a ls -> f a b = g a b) ->
+    fold_right f b ls = fold_right g b ls.
+  Admitted. (* TODO *)
+
+  (* TODO : move *)
+  Lemma fold_left_ext {A B} (f g : B -> A -> B) b ls :
+    (forall a b, In b ls -> f a b = g a b) ->
+    fold_left f ls b = fold_left g ls b.
+  Admitted. (* TODO *)
+
+  (* TODO : move *)
+  Lemma fold_left_nil {A B} (f : B -> A -> B) b :
+    fold_left f nil b = b.
+  Proof. reflexivity. Qed.
+  Hint Rewrite @fold_left_nil : push_fold_left.
+
+  (* TODO : move *)
+  Lemma Forall_map {A B} (P : B -> Prop) (f : A -> B) ls :
+    Forall P (map f ls) -> Forall (fun a => P (f a)) ls.
+  Admitted. (* TODO *)
+
+  (* TODO: move *)
+  Lemma abstract_reassign_pointer_change_concrete
+        abst conc conc' ptr attrs begin_index end_index :
+    Forall (fun root_ptr =>
+              index_sequences_to_pointer conc.(ptable_deref) ptr root_ptr
+              = index_sequences_to_pointer conc'.(ptable_deref) ptr root_ptr)
+            (hafnium_root_ptable :: map vm_root_ptable vms) ->
+    abstract_reassign_pointer abst conc ptr attrs begin_index end_index
+    = abstract_reassign_pointer abst conc' ptr attrs begin_index end_index.
+  Proof.
+    cbv [abstract_reassign_pointer].
+    repeat match goal with
+           | _ => progress basics
+           | _ => progress invert_list_properties
+           | H : _ |- _ => apply Forall_map in H; rewrite Forall_forall in H
+           | _ =>
+             rewrite abstract_reassign_pointer_for_entity_change_concrete
+               with (conc':=conc') by eauto
+           | _ => apply fold_right_ext
+           | _ => solve
+                    [auto using
+                          abstract_reassign_pointer_for_entity_change_concrete]
+           end.
+  Qed.
+
+  (* TODO : move *)
+  Lemma nth_default_skipn {A} (d:A) i j ls :
+    nth_default d (skipn i ls) j = nth_default d ls (j + i).
+  Admitted. (* TODO *)
+
+  (* TODO : move *)
+  Lemma nth_default_firstn_low {A} (d:A) i j ls :
+    j < i ->
+    nth_default d (firstn i ls) j = nth_default d ls j.
+  Admitted. (* TODO *)
+
+  Lemma mm_level_end_le a level : (a <= mm_level_end a level)%N.
+  Admitted. (* TODO *)
+
+  Definition is_root (level : nat) : Prop :=
+    exists flags, level = mm_max_level flags + 1.
+
+  Lemma root_pos level : is_root level -> 0 < level.
+  Proof. cbv [is_root]; simplify. Qed.
+
+  (* At the root level, every address has the same level_end *)
+  Lemma mm_level_end_root_eq root_level :
+    is_root root_level ->
+    forall a b, mm_level_end a root_level = mm_level_end b root_level.
+  Admitted. (* TODO *)
+
+  (* TODO : move *)
+  Lemma In_nth_default_firstn {A} (d:A) i j ls :
+    i < j ->
+    In (nth_default d ls i) (firstn j ls).
+  Admitted. (* TODO *)
+
+  (* TODO : move *)
+  Lemma In_nth_default_skipn {A} (d:A) i j ls :
+    j <= i ->
+    In (nth_default d ls i) (skipn j ls).
+  Admitted. (* TODO *)
+
+  (* TODO : move *)
+  Lemma In_nth_default_skipn_firstn {A} (d:A) i j k ls :
+    j <= i < k->
+    In (nth_default d ls i) (skipn j (firstn k ls)).
+  Admitted. (* TODO *)
+
+  (* TODO : move *)
+  (* has_uniform_attrs doesn't care if we reassign the pointer we started from *)
+  (* TODO : will need some kind of precondition saying the pointer doesn't repeat *)
+  Lemma has_uniform_attrs_reassign_pointer c ptr new_table t level attrs begin end_:
+    ~ pointer_in_table (ptable_deref c) ptr t ->
+    has_uniform_attrs (ptable_deref c) t level attrs begin end_ ->
+    has_uniform_attrs
+      (ptable_deref (reassign_pointer c ptr new_table))
+      t level attrs begin end_.
+  Admitted. (* TODO *)
+
+  (* TODO: move *)
+  (* has_uniform_attrs is trivially true for things before the start of the given
+     table; therefore, we can arbitrarily expand the range in that direction. *)
+  Lemma has_uniform_attrs_expand_range
+        deref table level attrs begin start end_ :
+    is_start_of_block start (S level) ->
+    (begin <= start)%N ->
+    has_uniform_attrs deref table level attrs start end_ ->
+    has_uniform_attrs deref table level attrs begin end_.
+  Admitted. (* TODO *)
+
+  (* TODO : move *)
+  (* TODO : probably will need preconditions about pointers being noncircular *)
+  Lemma abstract_reassign_pointer_root abst conc root_ptr attrs begin end_ :
+    represents
+      (fold_left
+         (fun abst t_ptr =>
+            abstract_reassign_pointer abst conc t_ptr attrs begin end_)
+         (mm_page_table_from_pa root_ptr)
+         abst)
+      conc ->
+    represents
+      (abstract_reassign_pointer abst conc (ptable_pointer_from_address root_ptr)
+                                 attrs begin end_)
+      conc.
+  Admitted. (* TODO *)
+
   (* TODO:
      This proof says only that if success = true and commit = true
      then the abstract state changed. We need two more proofs for full
@@ -216,6 +482,10 @@ Section Proofs.
      unchanged, and another saying that if success = true and commit =
      false, then success = true when the function is run again on the
      (unchanged) output state. *)
+  (* mm_level_end with level=root_level should be the end of the *root* ptable -- that means
+     mm_level_end begin root_level = mm_level_end end_ root_level *)
+  (* since abstract_reassign_pointer doesn't do anything if the
+  addresses given are out of range, we can reassign from root *)
   Lemma mm_map_root_represents_commit
         (conc : concrete_state)
         t begin end_ attrs root_level flags ppool :
@@ -225,100 +495,196 @@ Section Proofs.
     let ppool' := snd ret in
     let conc' := snd (fst ret) in
     let success := fst (fst ret) in
-    let t_ptrs := mm_page_table_from_pa t.(root) in
     let begin_index := mm_index begin root_level in
     let end_index := mm_index end_ root_level in
+    let t_ptrs :=
+        skipn begin_index
+              (firstn (S end_index) (mm_page_table_from_pa t.(root))) in
     success = true ->
     ((flags & MM_FLAG_COMMIT) != 0)%N = true ->
     (begin <= end_)%N ->
-    end_index < length t_ptrs ->
+    (* before calling mm_map_root, we have rounded end_ up to the nearest page,
+       and we have capped it to not go beyond the end of the table *)
+    end_index < length (mm_page_table_from_pa t.(root)) ->
+    (* we need to know we're actually at the root level *)
+    is_root root_level ->
+    (* nothing weird and circular going on with pointers *)
+    pointers_ok conc ppool ->
     forall abst,
       represents abst conc ->
-      represents (fold_right
-                    (fun t_ptr abst =>
+      represents (fold_left
+                    (fun abst t_ptr =>
                        abstract_reassign_pointer
-                         abst conc t_ptr attrs begin_index end_index)
-                    abst t_ptrs)
+                         abst conc t_ptr attrs begin end_)
+                    t_ptrs abst)
                  conc'.
   Proof.
     cbv zeta. cbv [mm_map_root].
     simplify.
 
-    let t_ptrs := constr:(mm_page_table_from_pa t.(root)) in
-    let start_begin := constr:(mm_index begin root_level) in
+    pose proof (root_pos root_level ltac:(auto)). 
+
+    let begin_index := constr:(mm_index begin root_level) in
+    let end_index := constr:(mm_index end_ root_level) in
+    let t_ptrs := constr:(skipn begin_index
+                                (firstn (S end_index)
+                                        (mm_page_table_from_pa t.(root)))) in
     match goal with
     | |- context [@while_loop _ ?iter ?cond ?start ?body] =>
       assert (mm_map_root_loop_invariant
-                abst conc t_ptrs start_begin attrs root_level
+                abst conc t_ptrs begin end_ attrs root_level
                 (@while_loop _ iter cond start body));
         [ apply while_loop_invariant | ]
     end;
-      cbv [mm_map_root_loop_invariant] in *; simplify;
-        repeat inversion_bool;
-        rewrite ?mm_map_level_represents.
-    { rewrite mm_index_start_of_next_block; reflexivity. }
-    { rewrite mm_index_start_of_next_block; reflexivity. }
-    { right.
-      cbn [firstn fold_right].
-      rewrite ?mm_map_level_represents.
-        cbv [mm_map_root_loop_invariant] in *; simplify.
-        right.
-          rewrite ?mm_map_level_represents
-    end.
-    Check while_loop_invariant.
-    { (* TODO: in this case, the map_level step failed, so we can't have returned success. *)
-      
-      Check reassign_pointer_represents.
-      Print mm_page_table_from_pa.
-      Check ptable_pointer_from_address.
-      SearchAbout s.
-    3:rewrite abstract_reassign_pointer_trivial; solver.
-    1-2: admit. (* mm_map_level layer *)
+      cbv [mm_map_root_loop_invariant] in *;
+      rewrite ?mm_map_level_represents; [ | | ].
+    { (* main case : prove invariant holds over step *)
 
-    match goal with
-    | H : represents (?f ?i) ?x |- represents (?f ?j) ?x =>
-      assert (i = j); [clear H | solver]
-    end.
+      (* conclude that mm_map_level succeeded *)
+      simplify; repeat inversion_bool; [ ].
+      right; rewrite !mm_map_level_represents.
 
+      (* split into the invariant clauses *)
+      simplify.
 
-    apply f_equal2; [|reflexivity].
-    apply Nnat.N2Nat.inj_iff.
-    match goal with
-    | |- context [@while_loop _ ?iter ?cond ?st ?body] =>
-      rewrite <- (while_loop_end_exact iter body
-                                       (fun '(_,_,_,failed,_) => negb failed)
-                                       (fun '(_,begin,_,_,_) => N.to_nat begin)
-                                       (N.to_nat end_)) with (start:=st);
-        simplify
-    end.
+      { (* table_index = mm_index begin root_level *)
+        rewrite mm_index_start_of_next_block; reflexivity. }
+      { (* start_begin <= begin *)
+        match goal with
+          |- (_ <= mm_start_of_next_block ?x _)%N => transitivity x; [solver|]
+        end.
+        admit. (* TODO : factor out mm_start_of_next_block proof saying it obeys le *) }
+      { (* begin <= mm_level_end end_ root_level *)
+        admit. (* TODO: factor out a lemma about mm_start_of_next_block saying that it won't skip over the level end *) }
+      { (* pointers_ok s ppool *)
+        admit. (* TODO : factor out mm_map_level proof *) }
+      { (* is_begin_or_block_start start_begin begin  *)
+        cbv [is_begin_or_block_start].
+        right. apply mm_start_of_next_block_is_start. }
+      { (* index sequences don't change *)
+        apply Forall_forall; intros.
+        apply Forall_forall; intros.
+        admit.
+        (* TODO: factor out a lemma about mm_map_level saying that reassigning the pointer is OK wrt existing pointer index sequences
+           (reasoning: mm_map_level is not going to add any new
+           pointers to the state unless it gets them from mpool, which
+           won't give out stuff that's already there -- probably will
+           require precondition saying mpool doesn't have any pointers
+           that are referenced from any roots) *) }
+      { (* represents step *)
+        pose proof (mm_level_end_root_eq root_level ltac:(assumption) begin end_).
 
-    {
-    repeat (f_equal;
-            try
-              (apply while_loop_proper_cond;
-               repeat match goal with
-                      | _ => progress basics
-                      | p : _ * _ |- _ => destruct p
-                      | _ => apply N.to_nat_ltb
-                      | _ => solver
-                      end)). }
-    6 : {
-    rewrite while_loop_proper_cond with
-        (cond':=fun '(_,begin,_,_,_) => N.to_nat begin <? N.to_nat end_) in * by
-        repeat match goal with
-               | _ => progress basics
-               | p : _ * _ |- _ => destruct p
-               | _ => apply N.to_nat_ltb
-               | _ => solver
-               end.
-    solver. }
+        (* find the current [begin] and assert that its index is in between the
+           start and end addresses' indices *)
+        match goal with
+        | H : is_begin_or_block_start _ ?x _ |- _ =>
+          assert (mm_index begin root_level <= mm_index x root_level)
+            by (apply mm_index_le_mono; solver);
+          assert (mm_index x root_level <= mm_index end_ root_level)
+            by (apply mm_index_le_mono; [ solver | ];
+                erewrite mm_level_end_root_eq by auto;
+                apply mm_level_end_le)
+        end.
 
-    { cbv [break continue] in *; solver. }
-    { admit. (* TODO: assume this about mm_start_of_next_block, that its results are > input *) }
-    { admit. (* TODO: assume this about mm_start_of_next_block, that it won't skip pages if end_ is aligned *) }
-    { apply Nat.leb_le. rewrite Nat.leb_compare.
-      rewrite <-Nnat.N2Nat.inj_compare. break_match; solver. }
-    { rewrite Nnat.N2Nat.inj_sub; solver. }
+        (* pull out S so we can rewrite about [firstn] *)
+        rewrite Nat.sub_succ_l by solver.
+
+        rewrite firstn_snoc with (d:=Datatypes.null_pointer)
+          by (autorewrite with push_length; lia).
+        rewrite fold_left_app.
+        cbn [fold_left].
+        cbv [nth_default_oobe Assumptions.Datatypes.ptable_pointer_oobe oob_value].
+
+        (* fix up the nth_default thing *)
+        rewrite nth_default_skipn.
+        rewrite nth_default_firstn_low by solver.
+        match goal with |- context [?a - ?b + ?b] =>
+                        replace (a - b + b) with a by omega end.
+
+        (* swap out starting concrete state for current one *)
+        match goal with
+          |- represents (abstract_reassign_pointer _ ?conc _ _ _ _) (reassign_pointer ?c _ _) =>
+          rewrite abstract_reassign_pointer_change_concrete with (conc':=c)
+            by
+              repeat match goal with
+                     | H : Forall _ _ |- _ => rewrite Forall_forall in H; apply H
+                     | _ => apply In_nth_default_skipn_firstn
+                     | _ => solver
+                     end
+        end.
+
+        apply reassign_pointer_represents with (level := root_level - 1).
+        { assumption. }
+        { apply has_uniform_attrs_reassign_pointer;
+            [ solve [auto using mm_map_level_noncircular] | ].
+          match goal with
+          | H : is_begin_or_block_start _ _ _ |- _ =>
+            destruct H as [H | H];
+              [ | replace root_level with (S (root_level - 1)) in H by solver ]
+          end.
+          { (* begin = n *)
+            simplify.
+            auto using mm_map_level_table_attrs. }
+          { eapply has_uniform_attrs_expand_range; try eassumption; [ ].
+            apply mm_map_level_table_attrs. } } } }
+    { (* invariant holds at start *)
+      right. simplify.
+      {  lia. }
+      {  erewrite mm_level_end_root_eq by eauto; apply mm_level_end_le. }
+      {  cbv [is_begin_or_block_start]; solver. }
+      { apply Forall_forall; intros.
+        apply Forall_forall; intros.
+        reflexivity. }
+      { rewrite Nat.sub_diag.
+        autorewrite with push_firstn push_fold_left.
+        auto. } }
+    { (* invariant implies correctness *)
+      repeat inversion_bool; simplify; [ ].
+      match goal with
+      | |- context [@while_loop _ ?iter ?cond ?st ?body] =>
+          assert (cond (@while_loop _ iter cond st body) = false);
+            [ apply (while_loop_completed iter cond body
+                                          (fun '(_,_,_,failed,_) => negb failed)
+                                          (fun '(_,begin,_,_,_) => N.to_nat begin)
+                                          (N.to_nat end_))
+            | remember (@while_loop _ iter cond st body) as RET]
+      end.
+
+      (* get rid of all but 2 goals *)
+      all:simplify.
+      all:try apply N.to_nat_ltb.
+      all:try apply Bool.negb_true_iff.
+      all:simplify.
+      all:try solve [rewrite ?Nnat.N2Nat.inj_sub; solver].
+
+      { admit. (* TODO: assume this about mm_start_of_next_block, that its results are > input *) }
+      {
+        match goal with |- context [while_loop _ _ ?body] => remember body as F end.
+        match goal with
+        | H : represents (fold_left ?f ?ls ?a) ?x
+          |- represents (fold_left ?f ?ls2 ?a) ?x =>
+          assert (ls = ls2); [clear H | solver ]
+        end.
+        (* prove lists are equal (i.e. the table index gets to the end of the list) *)
+
+        remember (snd (fst (fst (while_loop (fun '(_, begin0, _, _, _) => (begin0 <? end_)%N) (conc, begin, mm_index begin root_level, false, ppool) F)))) as IDX.
+        remember (snd (fst (fst (fst (while_loop (fun '(_, begin0, _, _, _) => (begin0 <? end_)%N) (conc, begin, mm_index begin root_level, false, ppool) F))))) as BEGIN.
+        remember (fst (fst (fst (fst (while_loop (fun '(_, begin0, _, _, _) => (begin0 <? end_)%N) (conc, begin, mm_index begin root_level, false, ppool) F))))) as CONC.
+        clear HeqBEGIN HeqCONC HeqIDX.
+
+        subst IDX.
+        
+        apply firstn_all2.
+        autorewrite with push_length.
+        rewrite Min.min_l by lia.
+        match goal with 
+        | H : (_ <? _)%N = false |- _ =>
+          apply N.ltb_ge in H;
+            apply mm_index_le_mono with (level:=root_level) in H; try solver
+        end.
+        assert (mm_index begin root_level <= mm_index end_ root_level) by admit.
+        apply Nat.sub_le_mono_r.
+        solver.
   Admitted.
 
   Lemma mm_ptable_identity_update_represents
